coq/SigmaHCOL/MemVecEq.v
@@ -1,0 +1,64 @@
+Require Import Helix.Util.VecUtil.
+Require Import Helix.Util.Matrix.
+Require Import Helix.Util.VecSetoid.
+Require Import Helix.Util.OptionSetoid.
+Require Import Helix.Util.Misc.
+Require Import Helix.Util.FinNat.
+Require Import Helix.SigmaHCOL.Rtheta.
+Require Import Helix.SigmaHCOL.SVector.
+Require Import Helix.SigmaHCOL.IndexFunctions.
+Require Import Helix.SigmaHCOL.Memory.
+Require Import Helix.SigmaHCOL.SigmaHCOLImpl.
+Require Import Helix.SigmaHCOL.SigmaHCOL.
+Require Import Helix.SigmaHCOL.SigmaHCOLMem.
+Require Import Helix.HCOL.HCOL. (* Presently for HOperator only. Consider moving it elsewhere *)
+Require Import Helix.Util.FinNatSet.
+Require Import Helix.Util.WriterMonadNoT.
+
+Require Import Coq.Logic.FunctionalExtensionality.
+Require Import Coq.Arith.Arith.
+Require Import Coq.Bool.Bool.
+Require Import Coq.Bool.BoolEq.
+Require Import Coq.Strings.String.
+Require Import Coq.Arith.Peano_dec.
+Require Import Coq.Logic.Decidable.
+
+Require Import Helix.Tactics.HelixTactics.
+Require Import Psatz.
+Require Import Omega.
+
+Require Import MathClasses.interfaces.abstract_algebra.
+Require Import MathClasses.orders.minmax MathClasses.interfaces.orders.
+Require Import MathClasses.theory.rings.
+Require Import MathClasses.implementations.peano_naturals.
+Require Import MathClasses.orders.orders.
+Require Import MathClasses.orders.semirings.
+Require Import MathClasses.theory.setoids.
+
+Require Import ExtLib.Structures.Monad.
+Require Import ExtLib.Structures.Monoid.
+
+Import Monoid.
+
+Import VectorNotations.
+Open Scope vector_scope.
+
+Definition svector_to_mem_block {fm} {n}:=
+  avector_to_mem_block ∘ @densify fm n.
+
+Global Instance mem_block_Equiv:
+  Equiv (mem_block) := mem_block_equiv.
+
+Class SHOperator_MemVecEq
+      {fm}
+      {i o: nat}
+      (f: @SHOperator fm i o)
+      `{facts: SHOperator_Facts _ _ _ f}
+  :=
+    {
+      mem_vec_preservation:
+        forall x,
+          Some (svector_to_mem_block (op fm f x)) =
+          mem_op fm f (svector_to_mem_block x)
+      ;
+    }.
